Safety5.v
@@ -1,0 +1,153 @@
+From Coq Require Import Arith.Arith.
+From Coq Require Import List.
+
+From Elo Require Import Array.
+From Elo Require Import Core0.
+From Elo Require Import Safety.
+
+
+
+
+
+
+
+
+
+
+
+
+
+
+
+Import ListNotations.
+
+Definition access_map m t (ads : list addr) :=
+  forall ad, access m t ad <-> In ad ads.
+
+(* Terms *)
+
+Lemma access_map_tm_nil : forall m,
+  access_map m TM_Nil [].
+Proof.
+  intros. split; intros F; inversion F.
+Qed.
+
+Lemma access_map_tm_num : forall m n,
+  access_map m (TM_Num n) [].
+Proof.
+  intros. split; intros F; inversion F.
+Qed.
+
+Lemma access_map_tm_loc : forall m ad ads,
+  access_map m (get TM_Nil m ad) ads ->
+  access_map m (TM_Loc ad) (ad :: ads).
+Proof.
+  intros * H ad'. specialize (H ad') as [? ?]. split; 
+  destruct (Nat.eq_dec ad ad'); subst; eauto using in_eq, access;
+  intros H'; inversion H'; subst; eauto using access, in_eq, in_cons.
+Qed.
+
+Lemma access_map_tm_new : forall m t ads,
+  access_map m t ads <-> access_map m (TM_New t) ads.
+Proof.
+  intros. split; intros H ad; specialize (H ad) as [? ?];
+  split; eauto using access, new_access.
+Qed.
+
+Lemma access_map_tm_load : forall m t ads,
+  access_map m t ads <-> access_map m (TM_Load t) ads.
+Proof.
+  intros. split; intros H ad; specialize (H ad) as [? ?];
+  split; eauto using access, load_access.
+Qed.
+
+Lemma access_map_tm_asg : forall m l r adsL adsR,
+  access_map m l adsL ->
+  access_map m r adsR ->
+  access_map m (TM_Asg l r) (adsL ++ adsR).
+Proof.
+  intros * Hl Hr ad.
+  specialize (Hl ad) as [? ?].
+  specialize (Hr ad) as [? ?].
+  split; intros H'.
+  - eapply asg_access in H' as [? | ?]; eauto using in_or_app.
+  - eapply in_app_or in H' as [? | ?]; eauto using access.
+Qed.
+
+Lemma access_map_tm_seq : forall m t1 t2 ads1 ads2,
+  access_map m t1 ads1 ->
+  access_map m t2 ads2 ->
+  access_map m (TM_Seq t1 t2) (ads1 ++ ads2).
+Proof.
+  intros * H1 H2 ad.
+  specialize (H1 ad) as [? ?].
+  specialize (H2 ad) as [? ?].
+  split; intros H'.
+  - eapply seq_access in H' as [? | ?]; eauto using in_or_app.
+  - eapply in_app_or in H' as [? | ?]; eauto using access.
+Qed.
+
+(* Effects *)
+
+Lemma access_map_eff_none : forall m m' t t' ads ads',
+  access_map m t ads ->
+  m / t ==[EF_None]==> m' / t' ->
+  access_map m' t' ads' ->
+  (forall ad, In ad ads' -> In ad ads).
+Proof.
+  assert (forall m t t' ad,
+    access m t' ad ->
+    t --[EF_None]--> t' ->
+    access m t ad). {
+      intros * Hacc Hstep.
+      remember EF_None as eff; induction Hstep; inversion Heqeff; subst;
+      eauto using access, load_access;
+      try (eapply asg_access in Hacc || eapply seq_access in Hacc);
+      specialize Hacc as [? | ?]; eauto using access.
+  }
+  intros * Hmap Hmstep Hmap'.
+  inversion Hmstep as [? ? ? Hstep | | |]; subst; clear Hmstep.
+  intros ? H'. eapply Hmap' in H'. eapply Hmap. eauto.
+Qed.
+
+Lemma access_map_eff_load : forall m m' t t' ad v ads ads',
+  access_map m t ads ->
+  m / t ==[EF_Load ad v]==> m' / t' ->
+  access_map m' t' ads' ->
+  (forall ad', In ad' ads' -> In ad' ads).
+Proof.
+  assert (forall m t t' ad ad',
+    access m t' ad ->
+    t --[EF_Load ad' (get TM_Nil m ad')]--> t' ->
+    access m t ad). {
+      intros * Hacc Hstep.
+      remember (EF_Load ad' (get TM_Nil m ad')) as eff;
+      induction Hstep; inversion Heqeff; subst;
+      eauto using access, load_access;
+      try (eapply asg_access in Hacc || eapply seq_access in Hacc);
+      specialize Hacc as [? | ?]; eauto using access.
+  }
+  intros * Hmap Hmstep Hmap'.
+  inversion Hmstep as [| | ? ? ? ? Hstep |]; subst; clear Hmstep.
+  intros ? H'. eapply Hmap' in H'. eapply Hmap. eauto.
+Qed.
+
+(*
+  TM_New
+  TM_Load
+  TM_Asg
+  TM_Seq
+  TM_Spawn
+*)
+(*
+  well_behaved_map m t map ->
+  m / t ==[eff]==> m' / t' ->
+  well_behaved_map m' t' map' ->
+
+  Se (eff = EF_None)  então (map' <= map)
+  Se (eff = EF_Alloc) então (map' >  map) -> (map' = (length m) :: map)
+  Se (eff = EF_Load)  então (map' <= map) -> (map' = map) \/ (map' = ad :: map)
+  Se (eff = EF_Store) então (map' <= map) -> (map' = map) \/ (map' = ad :: map)
+
+*)
+
